...결국 이 'tail_expr'을 구해야 하는 거잖아;;

src/02-Introduction-to-Semantics/Lecture02.ReflexiveTransitiveClosure.fst
@@ -2,157 +2,126 @@ module Lecture02.ReflexiveTransitiveClosure
 
 open Lecture02.BinaryRelation { (∈) } 
 module Br = Lecture02.BinaryRelation
-module Rule = Lecture02.InferenceRule
-module RuleBuilder = Lecture02.InferenceRule.Builder
 module L = FStar.List.Tot
 
-
 type step_t (state_t:eqtype) = (state_t & state_t)
-type small_step_relation_t (state_t:eqtype) = Br.binary_relation_t (Br.to_set state_t) (Br.to_set state_t)
-
-noeq
-type raw_builder_t 
-  #state_t (model_t:Type) (small_step_relation:small_step_relation_t state_t) =
-| ConclusionOnly: 
-    (to_conclusion:model_t -> (step_t state_t)) -> 
-    (raw_builder_t model_t small_step_relation)
-| AddPremise: 
-    (to_premise:model_t -> (step_t state_t)) ->
-    (raw_builder_t model_t small_step_relation) ->
-    (raw_builder_t model_t small_step_relation)
-
-
-let rec get_conclusion_from_raw
-  #state_t (#model_t:Type) (#small_step_relation:small_step_relation_t state_t)
-  (raw_builder:raw_builder_t model_t small_step_relation)
-  (model:model_t)
-  : Tot (step_t state_t) (decreases raw_builder) =
-  match raw_builder with
-  | ConclusionOnly tc -> tc model
-  | AddPremise tp pre_raw_builder -> get_conclusion_from_raw pre_raw_builder model
-
-let is_example
-  #state_t (#model_t:Type) (#small_step_relation:small_step_relation_t state_t)
-  (raw_builder:raw_builder_t model_t small_step_relation)
-  (model:model_t)
-  : prop =
-  match raw_builder with
-  | ConclusionOnly tc -> let s = tc model in (fst s) = (snd s)
-  | AddPremise tp pre_raw_builder ->
-  let s1 = tp model in
-  let s2 = get_conclusion_from_raw pre_raw_builder model in
-  let s3 = get_conclusion_from_raw raw_builder model in
-  (s1 ∈ small_step_relation) /\
-  ((fst s1) = (fst s3)) /\ ((snd s1) = (fst s2)) /\ ((snd s2) = (snd s3))
-
-let is_valid
-  #state_t (#model_t:Type) (#small_step_relation:small_step_relation_t state_t)
-  (raw_builder:raw_builder_t model_t small_step_relation)
-  : prop =
-  forall (model:model_t). (is_example raw_builder model)
-
-type builder_t 
-  #state_t (model_t:Type) (small_step_relation:small_step_relation_t state_t) =
-  x:(raw_builder_t model_t small_step_relation){is_valid x}
-
-private let rec to_rule_builder_core
-  #state_t (#model_t:Type) (#small_step_relation:small_step_relation_t state_t)
-  (raw_builder:raw_builder_t model_t small_step_relation) (lub_builder:builder_t model_t small_step_relation)
-  : Pure (RuleBuilder.t model_t) 
-    (requires (raw_builder == lub_builder) \/ (raw_builder << lub_builder))
-    (ensures fun r -> True)
-    (decreases raw_builder) =
-  match raw_builder with
-  | ConclusionOnly to_conclusion -> RuleBuilder.ConclusionOnly {
-      meta_proposition_t = step_t state_t;
-      apply = to_conclusion;
-      hold = fun x -> 
-        forall (model:model_t). (get_conclusion_from_raw lub_builder model) = (to_conclusion model)
-    }
-  | AddPremise to_premise pre_raw_builder ->
-    let new_premise : RuleBuilder.meta_proposition_schema_t model_t = {
-      meta_proposition_t = step_t state_t;
-      apply = to_premise;
-      hold = fun x -> (x ∈ small_step_relation)
-    } 
-    in
-    let pre_rule_builder = to_rule_builder_core pre_raw_builder lub_builder in
-    RuleBuilder.AddPremise new_premise pre_rule_builder
-
-let to_rule_builder
-  #state_t (#model_t:Type) (#small_step_relation:small_step_relation_t state_t)
-  (builder:builder_t model_t small_step_relation)
-  : Tot (RuleBuilder.t model_t) =
-  to_rule_builder_core builder builder
-
-let build
-  #state_t (#model_t:Type) (#small_step_relation:small_step_relation_t state_t)
-  (builder:builder_t model_t small_step_relation)
-  : Rule.t model_t =
-  RuleBuilder.build (to_rule_builder builder)
-
-open FStar.Tactics.V2
-let lemma_build 
-  #state_t (#model_t:Type) (#small_step_relation:small_step_relation_t state_t)
-  (builder:builder_t model_t small_step_relation)
-  : Lemma (Rule.is_valid (build builder)) =
-  //assert (Rule.is_valid (build builder)) by (dump "")
-  admit ()
-  (* 역시, 이게 그냥은 증명이 안 되네... *)
-
-type label_t =
-| Refl
-| Trans
-
-let get_label 
-  #state_t (#model_t:Type) (#small_step_relation:small_step_relation_t state_t)
-  (builder:builder_t model_t small_step_relation)
-  : label_t =
-  match builder with
-  | ConclusionOnly _ -> Refl
-  | AddPremise _ _ -> Trans
-
-
-(* goal: is_multi_step *)
-
-
-
+type small_step_relation_t (state_t:eqtype) = (state_t & state_t) -> bool
+//Br.binary_relation_t (Br.to_set state_t) (Br.to_set state_t)
 
 (*
-let is_rule 
-  (state_t:eqtype)
-  (x:Rule.t)
-  : prop =
-  (Rule.__proj__Mkt__item__label_t x == label_t) /\
-  (x.model_t == state_t)
+type expr_t #state_t (small_step_relation:small_step_relation_t state_t) =
+| ExprRefl: 
+    (conclusion:step_t state_t{(fst conclusion) = (snd conclusion)}) -> 
+    expr_t small_step_relation
+| ExprTrans: 
+    (premise0:step_t state_t{premise0 ∈ small_step_relation}) ->
+    (premise1:step_t state_t{(snd premise0) = (fst premise1)}) ->
+    (conclusion:step_t state_t{(fst premise0) = (fst conclusion) && (snd premise1) = (snd conclusion)}) ->
+    expr_t small_step_relation
+*)
 
-type rule_t (state_t:eqtype) =
-  x:Rule.t{is_rule state_t x}
+type expr_t (state_t:eqtype) =
+| ConclusionOnly: (step_t state_t) -> expr_t state_t
+| AddPremise: (step_t state_t) -> (expr_t state_t) -> expr_t state_t
 
-let get_refl_rule (state_t:eqtype) : rule_t state_t = {
-  label = Refl;
-  model_t = state_t;
-  premises = [];
-  conclusion = fun s -> s = s
-}
+let rec expr_count #state_t (expr:expr_t state_t)
+  : Tot pos (decreases expr) =
+  match expr with
+  | ConclusionOnly _ -> 1
+  | AddPremise _ pre_expr -> 1 + (expr_count pre_expr)
 
-let get_trans_rule 
-  (#state_t:eqtype)
-  (small_step_predicate:small_step_predicate_t state_t)
-  (pre_state:state_t)
-  (rule:rule_t state_t)
-  : (x:rule_t state_t{rule << x}) =
-  let p1 = small_step_predicate pre_state in
-  let next_premises = p1::rule.premises in
-  {
-    label = Trans;
-    model_t = state_t;
-    premises = next_premises;
-    conclusion = fun s -> (p1 s) /\ (p2 s)
-  }
+let get_first_step #state_t (expr:expr_t state_t)
+  : Tot (step_t state_t) (decreases expr) =
+  match expr with
+  | ConclusionOnly _0 -> _0
+  | AddPremise _0 _1 -> _0
 
+let rec get_last_step #state_t (expr:expr_t state_t)
+  : Tot (step_t state_t) (decreases expr) =
+  match expr with
+  | ConclusionOnly _0 -> _0
+  | AddPremise _0 _1 -> get_last_step _1
 
-let lemma_refl_rule (state_t:eqtype)
-  : Lemma (Rule.is_valid (get_refl_rule state_t)) =
-  ()
+private let rec is_valid_expr_core 
+  #state_t (expr:expr_t state_t) 
+  (small_step_relation:small_step_relation_t state_t)
+  (lub_expr:expr_t state_t{expr = lub_expr \/ expr << lub_expr})
+  : Tot bool (decreases expr) 
+  =
+  match expr with
+  | ConclusionOnly _0 -> 
+  begin
+    match expr = lub_expr with 
+    | true -> ((fst _0) = (snd _0))
+    | false -> ((fst _0) = (get_first_step lub_expr |> fst)) && ((snd _0) = (get_last_step lub_expr |> snd))
+  end
+  | AddPremise _0 pre_expr -> 
+    (_0 |> small_step_relation) && 
+    (is_valid_expr_core pre_expr small_step_relation lub_expr)
+
+let is_valid_expr #state_t (expr:expr_t state_t) (small_step_relation:small_step_relation_t state_t)
+  : bool =
+  is_valid_expr_core expr small_step_relation expr
+
+type valid_expr_t #state_t (small_step_relation:small_step_relation_t state_t) = 
+  x:expr_t state_t{is_valid_expr x small_step_relation}
+
+private let rec add_step_core 
+  #state_t (#small_step_relation:small_step_relation_t state_t)
+  (step:step_t state_t{small_step_relation step})
+  (expr:expr_t state_t)
+  (lub_expr:valid_expr_t small_step_relation{(expr = lub_expr \/ expr << lub_expr) /\ (snd step) = (fst (get_first_step lub_expr))})
+  (popped_steps:list (step_t state_t){small_step_relation step})
+  : Tot (expr_t state_t) 
+  (*
+    (requires (L.length popped_steps) = ((expr_count lub_expr) - (expr_count expr)))
+    (ensures fun r -> 
+      let r2 = L.fold_right (fun s e -> AddPremise s e) popped_steps r in
+      (is_valid_expr (AddPremise step r2) small_step_relation)
+    )
+  *)
+    (decreases expr) 
+  =
+  match expr with
+  | ConclusionOnly _0 -> 
+  begin
+    match expr = lub_expr with 
+    | true -> ConclusionOnly step
+    | false -> ConclusionOnly (step |> fst, get_last_step lub_expr |> snd)
+  end
+  | AddPremise _0 pre_expr -> AddPremise _0 (add_step_core step pre_expr lub_expr (_0::popped_steps))
+    
+let add_step 
+  #state_t (#small_step_relation:small_step_relation_t state_t)
+  (step:step_t state_t{small_step_relation step})
+  (expr:valid_expr_t small_step_relation{(snd step) = (fst (get_first_step expr))})
+  : Tot (valid_expr_t small_step_relation) =
+  let r = AddPremise step (add_step_core step expr expr []) in
+  assume (is_valid_expr r small_step_relation);
+  r
+
+type builder_t
+  #state_t (small_step_relation:small_step_relation_t state_t) 
+  : (expr:valid_expr_t small_step_relation) -> Type =
+| BuildNil:
+    (fix:state_t) ->
+    builder_t small_step_relation (ConclusionOnly (fix, fix))
+| BuildCons:
+    (head:step_t state_t{small_step_relation head}) ->
+    (#tail_expr:valid_expr_t small_step_relation{(snd head) = (fst (get_first_step tail_expr))}) ->
+    (tail:builder_t small_step_relation tail_expr) ->
+    builder_t small_step_relation (add_step head tail_expr)
+
+(*
+type builder_t 
+  #state_t (small_step_relation:small_step_relation_t state_t) 
+  : (expr_t small_step_relation) -> Type =
+| BuildNil:
+    (fix:state_t) ->
+    builder_t small_step_relation (ExprRefl (fix, fix))
+| BuildCons:
+    (head)
+    (_0:step_t state_t{_0 ∈ small_step_relation}) ->
+    (_1:state_t) ->
+    (_2:builder_t small_step_relation)
 *)
